concurrency/hack-hash-table/ApplicationResourceSpec.s.dfy
@@ -1,0 +1,69 @@
+include "../hack-concurrency-framework/ResourceSpec.s.dfy"
+include "MapSpec.s.dfy"
+
+abstract module ApplicationResourceSpec refines ResourceSpec {
+  import Ifc = MapIfc
+
+  function input_ticket(id: int, input: Ifc.Input) : R
+  function output_stub(id: int, output: Ifc.Output) : R
+
+  lemma NewTicketPreservesValid(r: R, id: int, input: Ifc.Input)
+  requires Valid(r)
+  ensures Valid(add(r, input_ticket(id, input)))
+
+  /*predicate Inv(s: R)
+
+  predicate NewTicket(s: R, s': R)
+  {
+    exists rid, input ::
+      s' == add(s, input_ticket(rid, input))
+  }
+
+  predicate ConsumeStub(s: R, s': R)
+  {
+    exists rid, output ::
+      s == add(s', output_stub(rid, output))
+  }
+
+  lemma UpdatePreservesInv(s: R, s': R)
+  requires Inv(s)
+  requires Update(s, s')
+  ensures Inv(s')
+
+  lemma NewTicketPreservesInv(s: R, s': R)
+  requires Inv(s)
+  requires NewTicket(s, s')
+  ensures Inv(s')
+
+  lemma ConsumeStubPreservesInv(s: R, s': R)
+  requires Inv(s)
+  requires ConsumeStub(s, s')
+  ensures Inv(s')*/
+
+  // refinement thm
+
+  /*
+  import AMS = AsyncSpec(MapIfc, MapSpec)
+
+  function I(m: R) : AMS.Variables
+
+  lemma InitRefines(s: R)
+  requires Init(s)
+  ensures AMS.Init(I(s))
+
+  lemma NextRefines(s: R, s': R)
+  requires Inv(s)
+  requires Next(s, s')
+  ensures AMS.Next(I(s), I(s'), AMS.Ifc.InternalOp)
+
+  lemma NewTicketRefines(s: R, s': R)
+  requires Inv(s)
+  requires s' == s + {query_ticket(id, key)}
+  ensures AMS.Next(I(s), I(s'), AMS.Ifc.Start(MapIfc.QueryRequest(key)))
+
+  lemma EraseStubRefines(s: R, s': R)
+  requires Inv(s)
+  requires s == s' + {query_stub(id, value)}
+  ensures AMS.Next(I(s), I(s'), AMS.Ifc.End(MapIfc.QueryResponse(value)))
+  */
+}
